ExamplePwMgrWithSSBFull.v
@@ -1,0 +1,10 @@
+Require Import Coq.FSets.FMapAVL Coq.FSets.FMapInterface.
+Require Import AESGCM SerializableMergableFMapInterface SerializableMergableFMapImplementation PwMgrUI ExamplePwMgrWithSSB.
+
+Module PreKVStore <: FMapInterface.Sfun String_as_SOT := FMapAVL.Make String_as_SOT.
+Module KVStore <: SerializableMergableMapInterface String_as_SOT := MakeSerializableMergableMap String_as_SOT PreKVStore.
+
+Module Export PwMgr := MakePwMgr KVStore AESGCM.
+
+Require Import ExtrOcamlBasic ExtrOcamlString.
+Extraction "ExamplePwMgrWithSSBFull" proc.
